progs/verif_sumarray.v
@@ -123,7 +123,7 @@ forward_while (sumarray_Inv a0 sh contents size)
 (* Prove that current precondition implies loop invariant *)
 unfold sumarray_Inv.
 apply exp_right with 0.
-entailer!. omega.
+entailer!.
 (* Prove that loop invariant implies typechecking condition *)
 entailer!.
 (* Prove that invariant && not loop-cond implies postcondition *)
@@ -137,8 +137,6 @@ forward. (* i++; *)
 unfold sumarray_Inv.
 apply exp_right with (Zsucc i0).
 entailer.
- omega.
- omega.
  simpl in H5. rewrite Int.signed_repr in H5 by repable_signed.
  rewrite fold_range_fact1 by omega.
  destruct (contents i0); inv H5. simpl. auto.
